proof/correctness768/avx2/Fq_avx2.ec
@@ -9,9 +9,6 @@ require import Fq MLKEM_Poly MLKEMFCLib.
 require import AVX2_Ops MLKEM_Poly_avx2_prevec.
 require import Montgomery16.
 
-(* require import NTT_Fq.
-require import Jkem768. *)
-
 import Fq MLKEM_Poly.
 import SignedReductions.
 
@@ -30,7 +27,38 @@ import ZModP.
 op lift_array16 (p: W16.t Array16.t) =
   Array16.map (fun x => (W16.to_sint x)) p.
 
-(* 
+module MLKEM_avx2_encdec = {
+  proc __fqmul_x16 (a b: W16.t Array16.t) : W16.t Array16.t = {
+    var i;
+    var t: W16.t;
+    var rd:W16.t Array16.t;
+    rd <- witness;
+    i <- 0;
+    while(i < 16) {
+      t <@ Fq.FQMUL_AVX.__fqmul(a.[i], b.[i]);
+      rd.[i] <- t;
+      i <- i + 1;
+    }
+
+    return (rd);
+  }
+
+  proc __red_x16 (r: W16.t Array16.t) : W16.t Array16.t = {
+    var i;
+    var t: W16.t;
+
+    i <- 0;
+    while(i < 16) {
+      t <@Jkem768.M.__barrett_reduce(r.[i]);
+      r.[i] <- t;
+      i <- i + 1;
+    }
+
+    return (r);
+  }
+}.
+
+
 lemma barret_red16x_corr_h:
   equiv [Mprevec.red16x ~ MLKEM_avx2_encdec.__red_x16 :
          ={r} /\
@@ -200,7 +228,6 @@ proof.
     apply W16.to_uint_eq; rewrite !of_uintK /=.
     smt().
 qed.
-*)
 
 lemma barret_red16x_ll:
   islossless Mprevec.red16x by proc; islossless.
@@ -211,7 +238,6 @@ lemma barret_red16x_corr _a:
           (forall k, 0 <= k < 16 => qx16.[k] = jqx16.[k]) /\
           (forall k, 0 <= k < 16 => vx16.[k] = jvx16.[k]) ==>
           forall k, 0 <= k < 16 => W16.to_sint res.[k] = BREDC _a.[k] 26] = 1%r.
-admitted. (* 
 proof.
 bypr => &m [#] /= H H0 H1.
 have -> : 1%r = 
@@ -276,7 +302,7 @@ case (k = 14); 1: by move => *; do 1!(rewrite Array16.set_neqiE 1,2:/#); rewrite
 case (k = 15); 1: by move => *; rewrite Array16.set_eqiE /#.
 by smt().
 qed.
-*)
+
 lemma barret_red16x_corr_hh _a:
   hoare [Mprevec.red16x:
           _a = lift_array16 r /\
@@ -298,7 +324,6 @@ have -> : Pr[Mprevec.red16x(r{m}, qx16{m}, vx16{m}) @ &m : true] = 1%r; last by 
 byphoare => //; apply barret_red16x_ll.
 qed.
 
-(* 
 lemma fqmulx16_corr_h:
   equiv [Mprevec.fqmulx16 ~ MLKEM_avx2_encdec.__fqmul_x16 :
          ={a, b} /\
@@ -551,7 +576,6 @@ rewrite modNz /= 1,2:/#.
   smt().
 
 qed.
-*)
 
 lemma fqmulx16_ll:
   islossless Mprevec.fqmulx16 by proc; islossless.
@@ -563,8 +587,6 @@ lemma fqmulx16_corr _a _b:
           (forall k, 0 <= k < 16 => qx16.[k] = W16.of_int 3329) /\
           (forall k, 0 <= k < 16 => qinvx16.[k] = W16.of_int (-3327)) ==>
           forall k, 0 <= k < 16 => to_sint res.[k] = SREDC (_a.[k] * _b.[k])] = 1%r.
-admitted.
-(* 
 proof.
 bypr => &m [#] /= H H0 H1 H2.
 have -> : 1%r = 
@@ -626,7 +648,8 @@ case (k = 14); 1: by move => *; do 1!(rewrite Array16.set_neqiE 1,2:/#); rewrite
 case (k = 15); 1: by move => *; rewrite Array16.set_eqiE /#.
 by smt().
 qed.
-*)
+
+
 lemma fqmulx16_corr_hh _a _b:
   hoare [Mprevec.fqmulx16 :
           _a = lift_array16 a /\
