proof/correctness768/avx2/MLKEM_KEM_avx2.ec
@@ -1,12 +1,12 @@
 require import AllCore IntDiv List.
 
-from JazzEC require import Jkem768_avx2.
+from JazzEC require import Jkem1024_avx2.
 
-from JazzEC require import Array1152 Array32 Array960 Array1184 Array1088 Array64 Array128.
+from JazzEC require import Array1152 Array32 Array1408 Array1568 Array1536 Array64 Array128 Array160 Array3168 WArray3168 WArray1568 WArray64 Array1600.
 from Jasmin require import JModel.
 
-from CryptoSpecs require import GFq Rq Sampling Serialization Symmetric VecMat InnerPKE768 MLKEM768 Correctness768.
-import Serialization768 Symmetric768 VecMat768.
+from CryptoSpecs require import GFq Rq Sampling Serialization Symmetric VecMat InnerPKE1024 MLKEM1024 Correctness1024.
+import Serialization1024 Symmetric1024 VecMat1024.
 require import Fq MLKEM_Poly MLKEM_PolyVec MLKEM_InnerPKE MLKEM_InnerPKE_avx2 MLKEMFCLib.
 
 import MLKEM_Poly.
@@ -16,417 +16,170 @@ require import MLKEM_keccak_avx2.
 
 lemma pack_inj : injective W8u8.pack8_t by apply (can_inj W8u8.pack8_t W8u8.unpack8 W8u8.pack8K).
 
-lemma mlkem_kem_correct_kg mem _pkp _skp  : 
-   equiv [Jkem768_avx2.M.__crypto_kem_keypair_jazz ~ MLKEM768.kg_derand : 
-       Glob.mem{1} = mem /\ to_uint pkp{1} = _pkp /\ to_uint skp{1} = _skp /\ 
+lemma mlkem_kem_correct_kg  : 
+   equiv [Jkem1024_avx2.M.__crypto_kem_keypair_jazz ~ MLKEM1024.kg_derand : 
         coins{2}.`1 = Array32.init(fun i => randomnessp{1}.[0 + i]) /\
-        coins{2}.`2 = Array32.init(fun i => randomnessp{1}.[32 + i]) /\
-       valid_disj_reg _pkp (384*3+32) _skp (384*3 + 384*3 + 32 + 32 + 32 + 32) 
+        coins{2}.`2 = Array32.init(fun i => randomnessp{1}.[32 + i])
         ==> 
-       touches2 Glob.mem{1} mem _pkp (384*3+32) _skp (384*3 + 384*3 + 32 + 32 + 32+ 32) /\
        let (pk,sk) = res{2} in let (t,rho) = pk in
-         sk.`1 = load_array1152 Glob.mem{1} _skp /\
-         sk.`2.`1 = load_array1152 Glob.mem{1} (_skp + 1152) /\
-         sk.`2.`2 = load_array32 Glob.mem{1} (_skp + 1152 + 1152) /\
-         sk.`3 = load_array32 Glob.mem{1} (_skp + 1152 + 1152 + 32) /\
-         sk.`4 = load_array32 Glob.mem{1} (_skp + 1152 + 1152 + 32 + 32) /\
-         t = load_array1152 Glob.mem{1} _pkp  /\
-         rho = load_array32 Glob.mem{1} (_pkp+1152)].
+         sk.`1 = Array1536.init (fun i => res{1}.`2.[i]) /\
+         sk.`2.`1 = Array1536.init (fun i =>  res{1}.`2.[i + 1536]) /\
+         sk.`2.`2 = Array32.init (fun i =>  res{1}.`2.[i + 1536 + 1536]) /\
+         sk.`3 = Array32.init (fun i => res{1}.`2.[i + 1536 + 1536 + 32]) /\
+         sk.`4 = Array32.init (fun i => res{1}.`2.[i + 1536 + 1536 + 32 + 32]) /\
+         t = Array1536.init (fun i => res{1}.`1.[i])  /\
+         rho = Array32.init (fun i => res{1}.`1.[i+1536])].
 proof.
 proc => /=.
-swap {1} 1 16.
-swap {1} [2..4] 17.
-seq 18 4 : (
-      z{2} = Array32.init(fun i => randomnessp{1}.[32 + i]) /\ 
-      to_uint skp{1} = _skp +  1152 + 1152 + 32 + 32 /\
-      valid_disj_reg _pkp (384*3+32) _skp (384*3 + 384*3 + 32 + 32 + 32 + 32) /\
-      touches2 Glob.mem{1} mem _pkp (384 * 3 + 32) _skp (384*3 + 384*3 + 32 + 32 + 32 + 32) /\
-      sk{2} = load_array1152 Glob.mem{1} _skp /\
-      pk{2}.`1 = load_array1152 Glob.mem{1} (_skp + 1152) /\
-      pk{2}.`2 = load_array32 Glob.mem{1} (_skp + 1152 + 1152) /\
-      hpk{2} = load_array32 Glob.mem{1} (_skp + 1152 + 1152 + 32) /\
-      pk{2}.`1 = load_array1152 Glob.mem{1} (_pkp) /\
-      pk{2}.`2 = load_array32 Glob.mem{1} (_pkp + 1152)
-); last first.
-+ while {1} (inc{1} = 4 /\
-       z{2} = Array32.init(fun i => randomnessp2{1}.[0 + i]) /\ 
-       to_uint skp{1} = _skp +  1152 + 1152 + 32 + 32 + i{1}*8 /\
-       valid_disj_reg _pkp (384*3+32) _skp (384*3 + 384*3 + 32 + 32 + 32 + 32) /\
-       touches2 Glob.mem{1} mem _pkp (384 * 3 + 32) _skp (384*3 + 384*3 + 32 + 32 + 32 + 32) /\
-       sk{2} = load_array1152 Glob.mem{1} _skp /\
-       pk{2}.`1 = load_array1152 Glob.mem{1} (_skp + 1152) /\
-       pk{2}.`2 = load_array32 Glob.mem{1} (_skp + 1152 + 1152) /\
-       hpk{2} = load_array32 Glob.mem{1} (_skp + 1152 + 1152 + 32) /\
-       pk{2}.`1 = load_array1152 Glob.mem{1} (_pkp) /\
-       pk{2}.`2 = load_array32 Glob.mem{1} (_pkp + 1152) /\
-       0 <= i{1} <= 4 /\ 
-       forall k, 0<=k<i{1} =>
-           loadW64 Glob.mem{1} (_skp + 2368 + k*8) =
-                 pack8_t (W8u8.Pack.init (fun i => z{2}.[k*8+i])))
-          (4 - i{1}).
-  + move => &m z0; auto => /> &hr; rewrite /touches2 /load_array1152 /load_array32 !tP => 
-       ?????? touch pk1vs pk2vs pk1v pk2v ??prev? ; rewrite !to_uintD_small /=.
-    + by smt(). 
-    do split; 1,9,12: by smt().
-    + by move => a H1 H2; rewrite /storeW64 /loadW64 /stores /= !get_set_neqE_s /#.
-    + by move => k kb; rewrite !initiE //= /storeW64 /loadW64 /stores /= !get_set_neqE_s /#.
-    + move => k kb; rewrite !initiE //= /storeW64 /loadW64 
-          /stores /= !get_set_neqE_s; 1..8: smt().     
-      by rewrite pk1vs // initiE //=.
-    + move => k kb; rewrite !initiE //= /storeW64 /loadW64 
-         /stores /= !get_set_neqE_s; 1..8: smt().     
-      by rewrite pk2vs // initiE //=.
-    + by move => k kb; rewrite !initiE //= /storeW64 /loadW64 
-         /stores /= !get_set_neqE_s;smt().
-    + move => k kb; rewrite !initiE //= /storeW64 /loadW64 
-         /stores /= !get_set_neqE_s; 1..8: smt(). 
-    by rewrite pk1v // initiE //=.
-    + move => k kb; rewrite !initiE //= /storeW64 /loadW64 
-        /stores /= !get_set_neqE_s; 1..8: smt(). 
-    by rewrite pk2v // initiE //=.
-    + by smt().
-    + move => k kbl kbh.
-      case (k < i{hr}).
-      + move => hk. 
-        rewrite /storeW64 /loadW64 /stores /=; congr. 
-        rewrite W8u8.Pack.packP => i ib; rewrite !initiE /=; 1,2: smt(). 
-        rewrite !get_set_neqE_s; 1..8: smt(). 
-        move : (prev k _); 1: by smt().
-        rewrite !initiE 1:/# /storeW64 /loadW64 /stores /=.
-        rewrite (inj_eq W8u8.pack8_t pack_inj) packP => H.
-        move : (H i _); 1: smt().
-        by rewrite !initiE //= initiE;  smt().
-     move => hk.
-     rewrite /storeW64 /loadW64 /stores /=.  
-     congr;rewrite W8u8.Pack.packP => ii iib; rewrite !initiE /=; 1..2: smt(). 
-     rewrite initiE /=; 1: smt(). 
-     rewrite WArray32.WArray32.get64E !pack8bE 1..8:/# !initiE 1..8:/# /= /init8.  
-      rewrite !WArray32.WArray32.initiE 1..8:/#.
-     by smt(get_set_neqE_s get_set_eqE_s).
+seq 4 0 : #pre;1: by auto.
+swap {1} 1 11. sp.
+seq 3 1 : (#{/~skcpa{1}}{~sk{1}}pre /\  
+   (forall k, 0 <= k < 1536 => sk{1}.[k] = sk{2}.[k]) /\
+   pk{2}.`1 = Array1536.init (fun i => pk{1}.[i])  /\
+   pk{2}.`2 = Array32.init (fun i => pk{1}.[i+1536])).
++ wp;call (mlkem_correct_kg_avx2);auto => /> &1 &2;rewrite !tP => ??;split.
+  + move => *; rewrite initiE 1:/#;smt(Array32.initiE).
+  move => ? rl [[rr11 rr12] rr2] /= [#];rewrite !tP => *; do split. 
+  + move => *; rewrite initiE 1:/# /= /#. 
+  + by move => *; rewrite initiE 1:/# /=; smt(Array1536.initiE).
+  + by move => *; rewrite initiE 1:/# /=; smt(Array32.initiE).
 
-  auto => />;move => ????????touch????; do split. 
-  + rewrite tP => k kb; rewrite !initiE 1..3:/# /=. 
-  +  smt().
-  +  smt().
-  move => memL iL skpL.  
-  split; 1: smt().
-  move => ???touch2????????store???. 
-  rewrite /load_array32 tP => k kb.
-  rewrite !initiE //=.
-  move : (store (k %/ 8) _); 1: smt().
-  rewrite /storeW64 /loadW64 /stores /load_array32 /=. 
-  rewrite (inj_eq W8u8.pack8_t pack_inj) packP => H.
-  move : (H (k %%8) _); 1: smt().
-  rewrite !initiE //=; 1,2:smt().
-  by rewrite !initiE //=; smt(). 
+seq 3 0 : (#pre /\
+ (forall (k : int), 0 <= k < 1568 => sk{1}.[k+1536] = pk{1}.[k])).
++ while {1} (#pre /\ inc{1} = 196 /\ 0 <= i{1} <= 196 /\
+    (forall k, 0 <= k < i{1}*8 =>
+        sk{1}.[k+1536] = pk{1}.[k])) (196-i{1}); last by auto => />; smt().
+  move => &2 ?; auto => /> &1 ?????????;do split;2..3,5..:smt().
+  + move => k kbl kbh;rewrite initiE 1:/# /= get8_set64_directE 1,2:/#.
+    case ((192 + i{1}) * 8 <= k < (192 + i{1}) * 8 + 8 ) => *.
+    +  rewrite /get64 /init8 /(\bits8) wordP => *.
+       by rewrite initiE 1:/# /=  /get64_direct /pack8_t initiE 1:/# /= initiE 1:/# /= initiE 1:/# /#. 
+    rewrite /get8 /init8 /(\bits8) wordP => *.
+    rewrite initiE 1:/# /= /#.
+  + move => k kbl kbh;rewrite initiE 1:/# /= get8_set64_directE 1,2:/#.
+    case ((192 + i{1}) * 8 <= k + 1536 < (192 + i{1}) * 8 + 8 ) => *.
+    +  rewrite /get64 /init8 /(\bits8) wordP => *.
+       by rewrite initiE 1:/# /=  /get64_direct /pack8_t initiE 1:/# /= initiE 1:/# /= initiE 1:/# /#. 
+    rewrite /get8 /init8 /(\bits8) wordP => *.
+    rewrite initiE 1:/# /= /#.
+    
+seq 2 1 : (#pre /\
+    (forall (k : int), 0 <= k < 32 => sk{1}.[k+1536 + 1568] = hpk{2}.[k])).
+wp;ecall {1} (sha3_256A_M1568_ph pk{1}).
++ auto => /> &1 &2 ??????; do split.
+  + move => *; rewrite initiE 1:/# /= /#. 
+  + by move => *; rewrite initiE 1:/# /=; smt(Array1536.initiE).
+  + by move => *; rewrite initiE 1:/# /=; smt(Array32.initiE).
 
-swap {2} 2 2. 
-swap {1} [2..3] 1; sp 4 1.
+seq  5 0 : (#pre /\
+    (forall (k : int), 0 <= k < 32 => sk{1}.[k+1536 + 1568 + 32] =randomnessp{1}.[k+32])).
++ while {1} (#pre /\ inc{1} = 4 /\ 0 <= i{1} <= 4 /\
+    (forall k, 0 <= k < i{1}*8 =>
+        sk{1}.[k+1536+1568+32] = randomnessp{1}.[k+32])) (4-i{1}); last by auto => /> /#.
++  move => &2 ?; auto => /> &1 ???????????;do split;4,5,7..:smt().
+  + move => k kbl kbh;rewrite initiE 1:/# /= get8_set64_directE 1,2:/#.
+    case ((392 + i{1}) * 8 <= k < (392 + i{1}) * 8 + 8 ) => *.
+    +  rewrite /get64 /init8 /(\bits8) wordP => *.
+       by rewrite initiE 1:/# /=  /get64_direct /pack8_t initiE 1:/# /= initiE 1:/# /= /#.
+    rewrite /get8 /init8 /(\bits8) wordP => *.
+    rewrite initiE 1:/# /= /#.
+  + move => k kbl kbh;rewrite initiE 1:/# /= get8_set64_directE 1,2:/#.
+    case ((392 + i{1}) * 8 <= k + 1536 < (392 + i{1}) * 8 + 8 ) => *.
+    +  rewrite /get64 /init8 /(\bits8) wordP => *.
+       by rewrite initiE 1:/# /=  /get64_direct /pack8_t initiE 1:/# /= initiE 1:/# /= /#. 
+    rewrite /get8 /init8 /(\bits8) wordP => *.
+    rewrite initiE 1:/# /= /#.
+  + move => k kbl kbh;rewrite initiE 1:/# /= get8_set64_directE 1,2:/#.
+    case ((392 + i{1}) * 8 <= k + 3104 < (392 + i{1}) * 8 + 8) => *.
+    +  rewrite /get64 /init8 /(\bits8) wordP => *.
+       by rewrite initiE 1:/# /=  /get64_direct /pack8_t initiE 1:/# /= initiE 1:/# /= /#. 
+    rewrite /get8 /init8 /(\bits8) wordP => *.
+    rewrite initiE 1:/# /= /#.
+  + move => k kbl kbh;rewrite initiE 1:/# /= get8_set64_directE 1,2:/#.
+    case (k < i{1}*8) => *. 
+    + rewrite ifF 1:/#. 
+      rewrite /get8 /init8 /(\bits8) wordP => kk kkb.
+      rewrite initiE 1:/# /= /#.
+    rewrite ifT 1:/#.
+    rewrite /get64 /init8 /(\bits8) wordP => kk kkb.
+    rewrite initiE 1:/# /=  /get64_direct /pack8_t initiE 1:/# /= initiE 1:/# /= initiE 1:/# /= /#.
 
-wp;conseq (_: _ ==>
-to_uint skp{1} = _skp + 2368 /\ 
-  touches2 Glob.mem{1} mem (_pkp) 1184 (_skp) 2432 /\
-  sk{2} = load_array1152 Glob.mem{1} (_skp) /\
-  pk{2}.`1 = load_array1152 Glob.mem{1} (_skp + 1152) /\
-  pk{2}.`2 = load_array32 Glob.mem{1} (_skp + 2304) /\
-  H_pk pk{2} = load_array32 Glob.mem{1} (_skp + 2336) /\
-  pk{2}.`1 = load_array1152 Glob.mem{1} ( _pkp) /\ 
-  pk{2}.`2 = load_array32 Glob.mem{1} (_pkp + 1152)); 1: by auto.
-
-seq 1 1 : (#{/~Glob.mem{1}=mem}pre /\
-  touches2 Glob.mem{1} mem _pkp 1184 _skp 2432 /\
-  sk{2} = load_array1152 Glob.mem{1} _skp /\
-  pk{2}.`1 = load_array1152 Glob.mem{1} _pkp /\ 
-  pk{2}.`2 = load_array32 Glob.mem{1} (_pkp + 1152)).
-call (mlkem_correct_kg_avx2 mem _pkp _skp).
-auto => /> &1 &2; rewrite /load_array1152 /load_array32 !tP /touches2 => ???????.
-do split; 1,2,3: smt().
-+ move =>  touch ????? [[resr11 resr12] resr2] memL touch2 /= [#]; rewrite !tP => r2 r11 r12. 
-  do split.
-  + by smt().
-  + by move => k kb;  move : (r2 k _) => //; rewrite !initiE //.
-  + by move => k kb;  move : (r11 k _) => //; rewrite !initiE //.
-  by move => k kb;  move : (r12 k _) => //; rewrite !initiE //.
-
-swap {1} 3 2.
-seq 8 0 : (#{/~to_uint skp{1} = _skp}pre /\
-   s_skp{1}=skp{1} /\
-   to_uint skp{1} = _skp + 3*384 + 3*384 + 32 /\
-   pk{2}.`1 = load_array1152 Glob.mem{1} (_skp + 1152) /\
-  pk{2}.`2 = load_array32 Glob.mem{1} (_skp+ 2304)
-).
-
-+ wp;while {1} (#{/~to_uint skp{1} = _skp}{~s_skp{1} = skp{1}}pre /\ 
-    inc{1} = (3 * 384 + 32) %/ 8 /\ 0<=i{1} <= inc{1} /\
-    to_uint skp{1} = _skp + 3*384 + i{1}*8 /\
-    (forall k, 0<= k < min (8 * i{1}) 1152  => 
-         pk{2}.`1.[k] = Glob.mem{1}.[_skp + 3*384 + k]) /\
-    (forall k, min (8 * i{1}) 1152 <= k < min (8 * i{1}) (1152 + 32) => 
-         pk{2}.`2.[k-1152] = Glob.mem{1}.[_skp + 3*384 +  k])) 
-    ((3 * 384 + 32) %/ 8 - i{1}).
-  move => &m z;auto => /> &hr. rewrite /load_array32 /load_array1152 !tP /touches2.
-  move => ???????touch pkv1 pkv2???prev1 prev2 ?;rewrite !to_uintD_small /=.
-  + by rewrite of_uintK /= modz_small /=; smt().
-  by smt().
-  do split; 5..7:smt().
-  + move => i ib ibb.
-    rewrite /storeW64 /loadW64 /stores  /=.
-    rewrite !get_set_neqE_s; 1..8:smt().
-    by smt(get_set_neqE_s get_set_eqE_s).
-  + move => i ib; rewrite !initiE //=.
-    rewrite /storeW64 /loadW64 /stores  /=.
-    rewrite !get_set_neqE_s; 1..8:smt().
-    by smt(get_set_neqE_s get_set_eqE_s).
-  + move => k kb; rewrite !initiE //=.
-    rewrite /storeW64 /loadW64 /stores  /=.
-    rewrite !get_set_neqE_s; 1..8:smt().
-    by move : (pkv1 k kb); rewrite initiE //=.
-  + move => k kb; rewrite !initiE //=.
-    rewrite /storeW64 /loadW64 /stores  /=.
-    rewrite !get_set_neqE_s; 1..8:smt().
-    by move : (pkv2 k kb); rewrite initiE //=.
-  + move => kk kkbl kkbh.
-    rewrite /storeW64 /loadW64 /stores  /=.
-    case (kk < i{hr} * 8).
-    + by move => *; rewrite !get_set_neqE_s; smt().
-    move => ?.
-    rewrite !of_uintK /= modz_small;1:smt().
-    move : (pkv1 kk _); 1: smt().
-    rewrite initiE /=; 1: smt().
-    by smt(get_set_neqE_s get_set_eqE_s).
-  + move => kk kkbl kkbh.
-    rewrite /storeW64 /loadW64 /stores  /=.
-    case (kk < i{hr} * 8).
-    + by move => *; rewrite !get_set_neqE_s; smt().
-    move => ?.
-    rewrite !of_uintK /= modz_small;1:smt().
-    move : (pkv2 (kk - 1152) _); 1: smt().
-    rewrite initiE /=; 1: smt().
-    by smt(get_set_neqE_s get_set_eqE_s).
-  + by smt().
-  auto => /> &1 &2; rewrite /load_array1152 /load_array32 !tP.
-  move =>  ??????????.
-  rewrite to_uintD_small /=; 1: by smt().
-  do split; 1..2: by smt(). 
-  move => meml il skpl.
-  rewrite !tP; split; 1: smt().
-  move => ??????????; do split; 1: smt().
-  + by move => *; rewrite initiE //= /#.
-  by move => *; rewrite initiE //= /#.
-   
-seq 2 0 : 
-(to_uint s_skp{1} = _skp + 2336 /\
-   valid_disj_reg _pkp 1184 _skp 2432 /\
-  touches2 Glob.mem{1} mem _pkp 1184 _skp 2432 /\
-  sk{2} = load_array1152 Glob.mem{1} _skp /\
-  pk{2}.`1 = load_array1152 Glob.mem{1} (_skp + 1152) /\
-  pk{2}.`2 = load_array32 Glob.mem{1} (_skp + 2304) /\
-  H_pk pk{2} = h_pk{1} /\ 
-  pk{2}.`1 = load_array1152 Glob.mem{1} _pkp /\ pk{2}.`2 = load_array32 Glob.mem{1} (_pkp + 1152)).
-
-ecall {1} (sha3_256A_M1184_ph (Glob.mem{1}) (_pkp)).
-inline *; auto => /> &1 &2; rewrite /touches /touches2 /load_array1152 /load_array32 !tP => ??????????? pk1v pk2v .
-+ move => i ib; congr; rewrite /H_pk; congr. 
-  by smt(Array32.initiE Array1152.initiE Array32.tP Array1152.tP).
-
-while {1} (#{/~to_uint skp{1} = _skp + 2336}pre /\ 0 <= i{1} <= 4 /\ to_uint skp{1} = _skp + 2336 + 8*i{1} /\ forall k, 0 <= k < i{1} * 8 => Glob.mem{1}.[_skp + 2336 + k] = ((H_pk pk{2})).[k]) (4 - i{1}).
-move => &m z; auto => /> &1 &2; rewrite /load_array1152 /load_array32 /touches2 !tP.
-move => ??????pkv1s pkv2s pkv1 pkv2 ??? prev ?. 
-rewrite !to_uintD_small /= 1:/#.
-do split.
-+ move => i ib ih.
-  rewrite /storeW64 /loadW64 /stores  /=. 
-  by smt(get_set_neqE_s get_set_eqE_s).
-+ move => i ib; rewrite !initiE //=.
-  rewrite /storeW64 /loadW64 /stores  /=. 
-  by smt(get_set_neqE_s get_set_eqE_s).
-+ move => i ib; rewrite !initiE //=.
-  rewrite /storeW64 /loadW64 /stores  /=.
-  rewrite !get_set_neqE_s;1..8:smt().
-  by move : (pkv1s i ib); rewrite initiE //=.
-+ move => i ib; rewrite !initiE //=.
-  rewrite /storeW64 /loadW64 /stores  /=.
-  rewrite !get_set_neqE_s;1..8:smt().
-  by move : (pkv2s i ib); rewrite initiE //=.
-+ move => i ib; rewrite !initiE //=.
-  rewrite /storeW64 /loadW64 /stores  /=.
-  rewrite !get_set_neqE_s;1..8:smt().
-  by move : (pkv1 i ib); rewrite initiE //=.
-+ move => i ib; rewrite !initiE //=.
-  rewrite /storeW64 /loadW64 /stores  /=.
-  rewrite !get_set_neqE_s;1..8:smt().
-  by move : (pkv2 i ib); rewrite initiE //=.
-+ by smt().
-+ by smt().
-+ by smt().
-+ move => k kbl kbh.
-  case (k < (i{1} * 8)).
-  + by move => kl;rewrite /storeW64 /loadW64 /stores  /=  !get_set_neqE_s;smt().
-  move => kh. rewrite /storeW64 /loadW64 /stores  /=. 
-  have -> :  (H_pk pk{m}).[k] = 
-              (WArray32.WArray32.get64 ((WArray32.WArray32.init8 ("_.[_]" (H_pk pk{m}))))%WArray32.WArray32 i{1})%WArray32.WArray32 \bits8 (k %% 8); last  by smt(get_set_neqE_s get_set_eqE_s).
-  rewrite /WArray32.WArray32.get64_direct.
-  by rewrite pack8bE 1:/# initiE /= 1:/# /WArray32.WArray32.init8 WArray32.WArray32.initiE /#.
-
-by smt().
-
-auto => /> &1 &2.
-rewrite /load_array1152 /load_array32 /touches2 !tP.
-move => ???????pkv1s pkv2s pkv1 pkv2. 
-do split. 
-+ move => i ib ih.
-  rewrite /storeW64 /loadW64 /stores  /=. 
-  by smt(get_set_neqE_s get_set_eqE_s).
-move => memL iL skL; do split; 1: by smt().
-move => *; split; 1: by smt().
-by rewrite tP => i ib; smt(Array32.initiE).
-
+auto => /> &1 &2; rewrite !tP => *;do split.
+  + move => *; rewrite initiE 1:/# /= /#. 
+  + by move => *; rewrite tP => *; rewrite initiE 1:/# /=  ; smt(Array1536.initiE).
+  + by move => *; rewrite tP => *; rewrite initiE 1:/# /=  ; smt(Array32.initiE).
+  + move => *; rewrite initiE 1:/# /=;smt(Array32.initiE).
+  + by move => *; rewrite initiE 1:/# /=; smt(Array32.initiE).
+ 
 qed.
 
+from JazzEC require import WArray32 Array4.
 
-lemma mlkem_kem_correct_enc mem _ctp _pkp _kp : 
-   equiv [Jkem768_avx2.M.__crypto_kem_enc_jazz ~ MLKEM768.enc_derand: 
-     valid_ptr _pkp (384*3 + 32) /\
-     valid_disj_reg _ctp (3*320+128) _kp (32) /\
-     Glob.mem{1} = mem /\ 
-     to_uint ctp{1} = _ctp /\ 
-     to_uint pkp{1} = _pkp /\
+lemma mlkem_kem_correct_enc  : 
+   equiv [Jkem1024_avx2.M.__crypto_kem_enc_jazz ~ MLKEM1024.enc_derand: 
      randomnessp{1} = coins{2} /\
-     to_uint shkp{1} = _kp /\
-     pk{2}.`1 = load_array1152 mem _pkp /\
-     pk{2}.`2 = load_array32 mem (_pkp + 3*384)
+     pk{2}.`1 = Array1536.init( fun i => pk{1}.[i]) /\
+     pk{2}.`2 = Array32.init( fun i => pk{1}.[1536+i])
        ==> 
-     touches2 Glob.mem{1} mem _ctp (3*320+128) _kp (32) /\
      let (c,k) = res{2} in
-     c.`1 = load_array960 Glob.mem{1} _ctp /\
-     c.`2 = load_array128 Glob.mem{1} (_ctp + 960) /\
-     k = load_array32 Glob.mem{1} _kp
+     c.`1 = Array1408.init (fun i => res{1}.`1.[i]) /\
+     c.`2 = Array160.init (fun i => res{1}.`1.[i+1408]) /\
+     k = res{1}.`2
 ].
-proc => /=.
-seq 13 4 : (#[/1:-2]post 
-      /\ valid_disj_reg _ctp 1088 _kp 32 
-      /\ to_uint s_shkp{1} = _kp 
-      /\ (forall k, 0<=k<32 => kr{1}.[k]=_K{2}.[k])); last first.
-+ while {1} (#[/1:-2]post
-      /\ inc{1} = 4 
-      /\ 0<=i{1}<=4 
-      /\ valid_disj_reg _ctp 1088 _kp 32 
-      /\ to_uint shkp{1} = _kp 
-      /\ (forall k, 0<=k<8*i{1} =>  _K{2}.[k] = (load_array32 Glob.mem{1} _kp).[k]) 
-      /\ (forall k, 0<=k<32 => kr{1}.[k]=_K{2}.[k])) (inc{1} - i{1}).
-  + auto => /> &hr H H0 H1 H2 H3 H4 H5 H6 H7 H8 H9 H10 H11;do split;4:smt().
-    + move : H;rewrite /touches2 => H a ab1 ab2. 
-      rewrite storeW64E get_storesE /=. 
-      by rewrite !to_uintD_small /= of_uintK /= modz_small /#.
-    + move : H0; rewrite /load_array960 !tP => H0 k kb.
-      rewrite initiE 1:/# /=.
-      rewrite storeW64E get_storesE /=. 
-      rewrite !to_uintD_small /= of_uintK /= modz_small 1..3:/# /=.
-      by have := H0 k kb; rewrite initiE 1:/# /= /#.
-    + move : H1; rewrite /load_array128 !tP => H1 k kb.
-      rewrite initiE 1:/# /=.
-      rewrite storeW64E get_storesE /=. 
-      rewrite !to_uintD_small /= of_uintK /= modz_small 1..3:/# /=.
-      by have := H1 k kb; rewrite initiE 1:/# /= /#. 
-    + by smt().
-    + move => k kbl kbh.
-      move : H9; rewrite /load_array32 => H9.
-      rewrite initiE 1:/# /=.
-      rewrite storeW64E get_storesE /=. 
-      rewrite !to_uintD_small /= of_uintK /= modz_small 1..3:/# /=.
-      case (k < 8 * i{hr}).
-      + move => kbb;have := H9 k _; 1: by smt().
-        by rewrite initiE 1:/# /= /#. 
-      rewrite !WArray64.WArray64.get64E.
-      by rewrite !pack8bE // !initiE //= /init8 !WArray64.WArray64.initiE /#.
-    by smt().
-  auto => /> &1 &2 ?????????;split;  1: by smt().
-  move => mm ii;do split => ???????; 1: smt().
-  by rewrite /load_array32 tP => kk kkb; smt(Array32.initiE).
-wp; call (mlkem_correct_enc_0_avx2 mem _ctp _pkp).
-wp; ecall {1} (sha3_512A_A64_ph buf{1}).
-wp; ecall {1} (sha3_256A_M1184_ph mem (_pkp)).
-seq 8 0 : (#pre /\ s_pkp{1} = pkp{1} /\ s_ctp{1} = ctp{1} /\  s_shkp{1} = shkp{1} /\ randomnessp{1} = Array32.init (fun i => buf{1}.[i])).
-+ sp ; conseq />.
-  while {1} (0<=i{1}<=inc{1} /\ inc{1} = 4 /\ randomnessp{1} = coins{2} /\  (forall k, 0<=k<i{1}*8 => randomnessp{1}.[k] = buf{1}.[k])) (inc{1} - i{1}); last first.
-  + auto => /> &1 &2 *; split; 1: by smt().  
-    move => buf i1; split; 1: smt(). 
-    by move => *; rewrite tP => k kn; rewrite initiE //= /#. 
-  move => &2 ?.
-  auto => /> &1 il ih premv ihh; do split; 1,2,4:smt().
-  move => k kl kh; rewrite initiE 1:/# /=.
-  rewrite WArray64.WArray64.get8_set64_directE 1..2:/#.
-  case (8 * i{1} <= k && k < 8 * i{1} + 8).
-  + move => *. 
-     rewrite WArray32.WArray32.get64E pack8bE 1:/# !initiE 1:/# /= /init8.  
-     by rewrite !WArray32.WArray32.initiE /#.
-  by move => *; rewrite /get8; rewrite WArray64.WArray64.initiE /#.
-auto  => /> &1 &2; rewrite /load_array1152 /load_array32 /load_array128 /load_array960 /touches2 /touches !tP.
-move => [#] ??????? pkv1 pkv2; do split.
-+ by move => i ib; rewrite !initiE /= /#.
-+ move => i ib; rewrite initiE /= 1:/# initiE /= 1:/# ifF 1:/#.
-  rewrite /G_mhpk; congr;congr;congr;rewrite tP => k kb.
-  + by rewrite !initiE 1,2,3:/# /= /H_msg ifF /#.
-  rewrite initiE 1:/# /= /H_pk. 
-  rewrite initiE 1:/# /= ifT 1:/#. 
-  congr;congr.
-  have -> : pk{2} = (pk{2}.`1,pk{2}.`2) by smt().
-  apply pw_eq; rewrite tP => kk kkb.
-  + by rewrite pkv1 /#.
-  by rewrite pkv2 /#. 
+proc => /=;sp 0 1.
+seq 6 2 : (#pre /\
+    Array32.init (fun (i : int) => kr{1}.[0 + i]) = _K{2} /\
+    Array32.init (fun (i : int) => kr{1}.[32 + i]) = r{2} /\
+    Array32.init (fun (i : int) => buf{1}.[i]) = m{2}).
+    wp; ecall {1} (sha3_512A_A64_ph buf{1}). 
+    wp; ecall {1} (sha3_256A_M1568_ph pk{1}). 
+    
+auto => /> &1 &2;rewrite !tP => *;do split => *.
++ rewrite initiE 1:/# /= initiE 1:/# /= ifT 1:/# /= /G_mhpk;congr;congr;congr.
+   + rewrite tP => *; rewrite  initiE 1:/# /= initiE 1:/# /= ifF 1:/# /= initiE 1:/# /= ifT 1:/# /= initiE 1:/# /get8 initiE 1:/# /= initiE 1:/# /= /get64_direct wordP => *.
+   rewrite /pack8_t /= /(\bits8) initiE 1:/# /= initiE 1:/# /= initiE 1:/# /= initiE 1:/# /= /#.
+   + rewrite tP => *; rewrite  initiE 1:/# /= initiE 1:/# /= ifT 1:/# /= initiE 1:/# /= /H_pk /SHA3_256_1568_32 get_of_list 1:/#;congr;congr;congr.
+      + congr;rewrite tP => *; rewrite initiE 1:/# /=;smt(Array1536.initiE). 
+      + congr;rewrite tP => *; rewrite initiE 1:/# /=;smt(Array32.initiE). 
 
-move => ?? [cR1 cR2] /= memR touch [-> ->]; do split.
-+ by move => a ? _; have := touch (a - to_uint ctp{1}); smt().
 
-rewrite /KDF /G_mhpk /H_msg /H_pk => k kb kbh. 
-rewrite !initiE //= 1:/# ifT 1:/#.
-congr. congr. congr. 
-+  rewrite tP => kk kkb.
-   by rewrite !initiE /= 1,2,3: /# ifF /#. 
-have -> : pk{2} = (pk{2}.`1,pk{2}.`2) by smt().
-rewrite tP => kk kkb. 
-pose xx := (SHA3_256_1184_32 (pk{2}.`1, pk{2}.`2)).[kk].
-rewrite !initiE 1:/# /= initiE 1:/# /= ifT 1:/#.
-rewrite /xx;congr;congr.
-apply pw_eq; rewrite tP => kkk kkkb.
-+ by rewrite pkv1 /#.
-by rewrite pkv2 /#. 
++ rewrite initiE 1:/# /= initiE 1:/# /= ifF 1:/# /= /G_mhpk;congr;congr;
+congr.
+   + rewrite tP => *; rewrite  initiE 1:/# /= initiE 1:/# /= ifF 1:/# /= initiE 1:/# /= ifT 1:/# /= initiE 1:/# /get8 initiE 1:/# /= initiE 1:/# /= /get64_direct wordP => *.
+   rewrite /pack8_t /= /(\bits8) initiE 1:/# /= initiE 1:/# /= initiE 1:/# /= initiE 1:/# /= /#.
+   + rewrite tP => *; rewrite  initiE 1:/# /= initiE 1:/# /= ifT 1:/# /= initiE 1:/# /= /H_pk /SHA3_256_1568_32 get_of_list 1:/#;congr;congr;congr.
+      + congr;rewrite tP => *; rewrite initiE 1:/# /=;smt(Array1536.initiE). 
+      + congr;rewrite tP => *; rewrite initiE 1:/# /=;smt(Array32.initiE). 
+
++ rewrite initiE 1:/# /= initiE 1:/# /= ifF 1:/# /= initiE 1:/# /= ifT 1:/# /= initiE 1:/# /= /get8 initiE 1:/# /= initiE 1:/# /= /get64_direct wordP => *.
+   rewrite /pack8_t /= /(\bits8) initiE 1:/# /= initiE 1:/# /= initiE 1:/# /= initiE 1:/# /= /#.
+
+wp; ecall (mlkem_correct_enc_1_avx2 pk{1}) => /=.
+auto => /> &1 &2; rewrite tP => *;do split;1:smt().
+move => ? r0 [r111 r12] /= [#]; rewrite !tP => *;do split;1,2:smt().
+move => *;rewrite !initiE 1,2:/# /= /get8 initiE 1:/# /= initiE 1:/# /= /get64_direct wordP => *.
+   rewrite /pack8_t /= /(\bits8) initiE 1:/# /= initiE 1:/# /= initiE 1:/# /= initiE 1:/# /= initiE 1:/# /= /#. 
 qed.
 
 require import StdOrder. 
 import IntOrder.
-
-lemma verify_correct_h mem (_ctp : int) ctp1 :
-  hoare [Jkem768_avx2.M.__verify : 
-             Glob.mem = mem /\ valid_ptr _ctp 1088 /\
-             to_uint ctp = _ctp /\ ctpc = ctp1 ==>
-             Glob.mem = mem /\
-             (Array1088.init (fun i => loadW8 mem (_ctp + i)) = ctp1 => 
-                       res = W64.of_int 0) /\
-             (Array1088.init (fun i => loadW8 mem (_ctp + i)) <> ctp1 => 
-                       res = W64.of_int 1)].
+lemma verify_correct_h _ct _ct1 :
+  hoare [Jkem1024_avx2.M.__verify : 
+             ct = _ct /\ ctpc =_ct1 ==>
+             (_ct = _ct1 => res = W64.of_int 0) /\
+             (_ct <> _ct1 => res = W64.of_int 1) 
+].
 proc => /=.
-seq 8 : (#post); last first.
-wp. conseq />. while(i=1088 /\ inc=1088 /\ #pre); 1: by auto => />. 
-+ (*conseq />; 1: by smt(). *)
-  conseq />; first by move => /> *; split; smt().
-  auto => />.  
-  move => &hr H H1 _cnd H2 H3.
-  split. 
-  + by move => H4; move : (H2 H4) => -> /=; rewrite W64.WRingA.oppr0 to_uint_eq W64.shr_div_le //.
-  + move => H5; move : (H3 H5) => -> /=; rewrite W64.minus_one /= wordP => i ib.
-    by rewrite /(`>>`) shrwE ib /= /(W64.one) /= /bits2w /= initiE //= /int2bs /= /mkseq /= -iotaredE /= /#. 
 
-wp; while (#pre /\ 0 <= i{hr} <= 34 /\ inc{hr} = 34 /\ 0<=to_uint cnd<256 /\
+wp; while (#pre /\ 0 <= i{hr} <= 49 /\ inc{hr} = 49 /\ 0<=to_uint cnd<256 /\
            (to_uint h{hr} = 0 <=> 
-            forall k, 0 <= k < i{hr}*32 => loadW8 mem (_ctp + k) = ctp1.[k])); last first.
-+ auto => /> &hr ??; split; 1: by smt().
+            (forall k, 0 <= k < i{hr}*32 => ct.[k] = ctpc.[k]))); last first.
++ auto => />; split; 1: by smt().
   move => h i ??? [HL HR]; split; last first.
   + rewrite tP => H1.
     rewrite /VPTEST_256 /= /ZF_of /= ifT //.
     move : H1; rewrite negb_forall /= => [[k H]]. 
     move : H; rewrite negb_imply  /= => [# H1 H2 H3].
-    rewrite initiE //= in H3.
     rewrite implybE in HL; elim HL; smt(to_uint0). 
 
   + rewrite tP => H1.
@@ -434,13 +187,11 @@ wp; while (#pre /\ 0 <= i{hr} <= 34 /\ inc{hr} = 34 /\ 0<=to_uint cnd<256 /\
     rewrite implybE in HR; elim HR.
     +  rewrite negb_forall /= => [[k H]].  
        move : H; rewrite negb_imply  /= => [# H2 H3 H4].
-       smt(Array1088.initiE).
+       smt(Array1568.initiE).
     smt(W256.to_uint_eq W256.to_uint0).
 
-auto => /> &hr ?????? [HL HR] ?.
-pose x := 
-      ((WArray1088.WArray1088.get256 ((WArray1088.WArray1088.init8 ("_.[_]" ctp1)))%WArray1088.WArray1088 i{hr})) `^`
-        loadW256 mem (to_uint (ctp{hr} + (of_int (32 * i{hr}))%W64)).
+auto => /> &hr ???? [HL HR] ?.
+pose x := get256 (WArray1568.init8 ("_.[_]" _ct1)) i{hr} `^` get256 (WArray1568.init8 ("_.[_]" _ct)) i{hr}.
 do split; 1..2: by smt().
 + move => H0 k kbl kbh.
 
@@ -462,9 +213,7 @@ do split; 1..2: by smt().
   move : (H2 ((k - i{hr} * 32) * 8 + j) _). smt().
   rewrite !pack32wE /=; 1,2: smt().
   rewrite !initiE /=; 1,2: smt().
-  rewrite to_uintD_small /=; 1: by rewrite /= of_uintK /=; by smt(W64.to_uint_cmp).  
-  rewrite /= of_uintK /= (modz_small _  18446744073709551616) 1:/#.
-  rewrite WArray1088.WArray1088.initiE 1:/# /=. smt().
+  rewrite !WArray1568.initiE 1,2:/# /=; smt().
 
 move => H0.
 have -> : h{hr} = W256.zero by rewrite to_uint_eq /= /#.
@@ -477,55 +226,33 @@ have -> : xx = yy; last by rewrite xorwK_s //.
 rewrite /xx /yy wordP => j jb.
   rewrite !pack32wE /=; 1,2: smt().
   rewrite !initiE /=; 1,2: smt().
-  rewrite to_uintD_small /=; 1: by rewrite /= of_uintK /=; by smt(W64.to_uint_cmp).  
-  rewrite /= of_uintK /= (modz_small _  18446744073709551616) 1:/#.
-  rewrite WArray1088.WArray1088.initiE 1:/# /=. smt().
+  rewrite !WArray1568.initiE 1,2:/# /=; smt().
 qed.
 
-lemma verify_ll : islossless Jkem768_avx2.M.__verify.
+lemma verify_ll : islossless Jkem1024_avx2.M.__verify.
 proc.
-seq 8 : (#post) => //; last first.
-wp. conseq />. while(i=1088 /\ inc=1088 /\ #pre) (1088 - inc); 1,2:   by auto => />. 
 wp.
-while (0 <= i{hr} <= 34 /\ inc{hr} = 34) (34 - i{hr}).
+while (0 <= i{hr} <= 49 /\ inc{hr} = 49) (49 - i{hr}).
 auto => /> /#.
 auto => /> /#. 
 qed.
 
-lemma verify_correct mem (_ctp : int) ctp1 :
-  phoare [Jkem768_avx2.M.__verify : 
-             Glob.mem = mem /\ valid_ptr _ctp 1088 /\
-             to_uint ctp = _ctp /\ ctpc = ctp1 ==>
-             Glob.mem = mem /\
-             (Array1088.init (fun i => loadW8 mem (_ctp + i)) = ctp1 => 
-                       res = W64.of_int 0) /\
-             (Array1088.init (fun i => loadW8 mem (_ctp + i)) <> ctp1 => 
-                       res = W64.of_int 1)] = 1%r 
-   by conseq verify_ll (verify_correct_h mem _ctp ctp1).
+lemma verify_correct  _ct _ct1 :
+  phoare [Jkem1024_avx2.M.__verify : 
+              ct = _ct /\ ctpc =_ct1 ==>
+             (_ct = _ct1 => res = W64.of_int 0) /\
+             (_ct <> _ct1 => res = W64.of_int 1) ] = 1%r 
+   by conseq verify_ll (verify_correct_h  _ct _ct1).
 
-lemma cmov_correct_h _dst _src _cnd mem:
-   hoare [Jkem768_avx2.M.__cmov : 
-             Glob.mem = mem /\ valid_ptr _dst 32 /\
-             src = _src /\ cnd = _cnd /\ to_uint dst = _dst ==>
-             touches mem Glob.mem _dst 32 /\
-             (_cnd = W64.of_int 0 => 
-               (Array32.init (fun i => loadW8 Glob.mem (_dst + i))) = _src) /\
-             (_cnd = W64.of_int 1 => 
-               (Array32.init (fun i => loadW8 Glob.mem (_dst + i))) = 
-                (Array32.init (fun i => loadW8 mem (_dst + i))))].
+lemma cmov_correct_h _dst _src _cnd :
+   hoare [Jkem1024_avx2.M.__cmov : 
+             src = _src /\ cnd = _cnd /\  dst = _dst ==>
+             (_cnd = W64.of_int 0 => res = _src)/\
+             (_cnd = W64.of_int 1 => res = _dst)].
 proc => /=.
 seq 1 : (#{/~cnd}pre /\ (_cnd = W64.zero => cnd = W64.zero) /\
                 (_cnd = W64.one => cnd = W64.onew));
-  1: by auto => /> &1 ?? /=; split; [ by ring | by rewrite W64.minus_one /=].
-
-unroll ^while.
-
-seq 5 : (#post /\ inc{hr}= 1 /\ i{hr}=1); last first.
-+ wp; conseq />; while(i=1 /\ inc=1 /\ #pre); auto => /> /#. 
-
-rcondt 5; 1: by move => *; auto => />.
-
-auto => /> &hr H H0 H1 H2.
+  1: by auto => />   /=; split; [ by ring | by rewrite W64.minus_one /=].
 
 have msb1 : forall i,  0 <= i < 8 => msb (W64.onew \bits8 i) = true.
 + move => i ib; rewrite /msb /=.
@@ -541,199 +268,151 @@ have msb0 : forall i, 0 <= i <8 => msb (W64.zero \bits8 i) = false.
     rewrite zerowE  /= bits8iE //= /#.
   by rewrite to_uint0 /=.
 
-do split.
-+ rewrite /touches => a ab.
-  rewrite /storeW256 /loadW256 /loads /stores /=.
-  by do 32!(rewrite get_setE ifF 1:/#);smt().
+auto => /> &hr H H0;split.
 
-+ move =>czero; move : (H1 czero) => -> /=;rewrite tP => k kb.
-rewrite initiE //= /storeW256 /=.
-have HH : forall ii, 0<=ii <32 => BLENDV_32u8 ((WArray32.WArray32.get256_direct ((WArray32.WArray32.init8 ("_.[_]" _src))) 0))
-          (loadW256 mem (to_uint dst{hr})) (VPBROADCAST_4u64 W64.zero) \bits8
-        ii = _src.[ii]; last first. 
-+ rewrite !HH //=.
-  by rewrite /loadW8 /stores /= !get_setE /= /#.
++ move =>czero; move : (H czero) => -> /=;rewrite tP => k kb.
+rewrite !initiE //= kb /=.
+have HH : forall ii, 0<=ii <32 => VPBLENDVB_256 ((WArray32.get256_direct ((WArray32.init8 ("_.[_]" _src))) 0))
+          (get256_direct (WArray32.init8 ("_.[_]" _dst)) 0) (VPBROADCAST_4u64 W64.zero) \bits8
+        ii = _src.[ii]; last by rewrite HH. 
 move => ii iib.
 rewrite /get256_direct /init8 /loadW256 /loadW8 /= wordP => i ib.
-rewrite /BLENDV_32u8 /VPBLENDVB_256 /VPBROADCAST_4u64 /(\bits8) -iotaredE /= /BLENDV_16u8 /VPBLENDVB_128 /= !msb0 //=  initiE //=.
+rewrite /VPBLENDVB_256 /VPBROADCAST_4u64 /(\bits8) -iotaredE /= /VPBLENDVB_128 /= !msb0 //=  initiE //=.
 rewrite pack32E initiE /= 1:/# /of_list initiE /= /#.
  
-+ move =>cone; move : (H2 cone) => -> /=;rewrite tP => k kb.
-rewrite initiE //= /storeW256 /=.
-have HH : forall ii, 0<=ii <32 => BLENDV_32u8 ((WArray32.WArray32.get256_direct ((WArray32.WArray32.init8 ("_.[_]" _src))) 0))
-        (loadW256 mem (to_uint dst{hr})) (VPBROADCAST_4u64 W64.onew) \bits8
-              ii = ((init (fun (i0 : int) => loadW8 mem (to_uint dst{hr} + i0))))%Array32.[ii]; last first. 
-+ rewrite !HH //=.
-  by rewrite initiE //= /loadW8 /stores /= !get_setE /= /#.
++ move =>cone; move : (H0 cone) => -> /=;rewrite tP => k kb.
+rewrite initiE //= /storeW256 kb /=.
+have HH : forall ii, 0<=ii <32 => VPBLENDVB_256 ((WArray32.get256_direct ((WArray32.init8 ("_.[_]" _src))) 0))
+        (get256_direct (WArray32.init8 ("_.[_]" _dst)) 0) (VPBROADCAST_4u64 W64.onew) \bits8
+              ii = _dst.[ii]; last by rewrite HH. 
 move => ii iib.
 rewrite /get256_direct /init8 /loadW256 /loadW8 /= wordP => i ib.
-rewrite /BLENDV_32u8 /VPBLENDVB_256 /VPBROADCAST_4u64 /(\bits8) -iotaredE /= /BLENDV_16u8 /VPBLENDVB_128 /= !msb1 //=  initiE //=.
+rewrite /VPBLENDVB_256 /VPBROADCAST_4u64 /(\bits8) -iotaredE /= /VPBLENDVB_128 /= !msb1 //=  initiE //=.
 by rewrite pack32E initiE /= 1:/# /of_list !initiE /= /#.
 qed.
 
-lemma cmov_ll : islossless Jkem768_avx2.M.__cmov.
-proc => /=.
-unroll 6.
-
-+ wp; conseq />; while(i=1 /\ inc=1 /\ #pre) (1-i); auto => /> /#. 
-qed.
+lemma cmov_ll : islossless Jkem1024_avx2.M.__cmov by islossless.
 
 
-lemma cmov_correct _dst _src _cnd mem:
-   phoare [Jkem768_avx2.M.__cmov : 
-             Glob.mem = mem /\ valid_ptr _dst 32 /\
-             src = _src /\ cnd = _cnd /\ to_uint dst = _dst ==>
-             touches mem Glob.mem _dst 32 /\
-             (_cnd = W64.of_int 0 => 
-               (Array32.init (fun i => loadW8 Glob.mem (_dst + i))) = _src) /\
-             (_cnd = W64.of_int 1 => 
-               (Array32.init (fun i => loadW8 Glob.mem (_dst + i))) = 
-                (Array32.init (fun i => loadW8 mem (_dst + i))))] = 1%r
-    by conseq cmov_ll (cmov_correct_h _dst _src _cnd mem).
+lemma cmov_correct _dst _src _cnd:
+   phoare [Jkem1024_avx2.M.__cmov : 
+            src = _src /\ cnd = _cnd /\  dst = _dst ==>
+             (_cnd = W64.of_int 0 => res = _src)/\
+             (_cnd = W64.of_int 1 => res = _dst)] = 1%r
+    by conseq cmov_ll (cmov_correct_h _dst _src _cnd).
 
-lemma mlkem_kem_correct_dec mem _ctp _skp _shkp : 
-   equiv [Jkem768_avx2.M.__crypto_kem_dec_jazz ~ MLKEM768.dec: 
-     valid_ptr _ctp (3*320+128) /\
-     valid_ptr _skp (384*3 + 384*3 + 32 + 32 + 32+ 32) /\
-     valid_ptr _shkp 32 /\
-     Glob.mem{1} = mem /\ 
-     to_uint shkp{1} = _shkp /\
-     to_uint ctp{1} = _ctp /\
-     to_uint skp{1} = _skp /\
-     sk{2}.`1 = load_array1152 Glob.mem{1} _skp /\
-     sk{2}.`2.`1 = load_array1152 Glob.mem{1} (_skp + 1152) /\
-     sk{2}.`2.`2 = load_array32 Glob.mem{1} (_skp + 1152 + 1152) /\
-     sk{2}.`3 = load_array32 Glob.mem{1} (_skp + 1152 + 1152 + 32) /\
-     sk{2}.`4 = load_array32 Glob.mem{1} (_skp + 1152 + 1152 + 32 + 32) /\
+from JazzEC require import Array196.
+lemma mlkem_kem_correct_dec  : 
+   equiv [Jkem1024_avx2.M.__crypto_kem_dec_jazz ~ MLKEM1024.dec: 
+     sk{2}.`1 = Array1536.init (fun i =>  sk{1}.[i]) /\
+     sk{2}.`2.`1 = Array1536.init (fun i => sk{1}.[i + 1536]) /\
+     sk{2}.`2.`2 = Array32.init (fun i =>  sk{1}.[i + 1536 + 1536]) /\
+     sk{2}.`3 = Array32.init (fun i => sk{1}.[i + 1536 + 1536 + 32]) /\
+     sk{2}.`4 = Array32.init (fun i => sk{1}.[i+ 1536 + 1536 + 32 + 32]) /\
      let (c1,c2) = cph{2} in
-       c1 = load_array960 Glob.mem{1} _ctp /\
-       c2 = load_array128 Glob.mem{1} (_ctp + 960)
-       ==> 
-     touches Glob.mem{1} mem _shkp 32 /\
-     res{2} = load_array32 Glob.mem{1} _shkp
-].
-proc => /=. sp 0 1. swap {1} [4..5] 12.
+       c1 = Array1408.init(fun i => ct{1}.[i]) /\
+       c2 = Array160.init(fun i => ct{1}.[i + 1408])
+       ==> ={res}].
+proc => /=. sp 0 1. swap {1} [4..5] 6.
 
 seq 4 1 : (#pre /\ aux{1} = m{2}); 
-  1: by call (mlkem_correct_dec mem _ctp _skp); 1: by auto => /> /#.
+  1: by call (mlkem_correct_dec); 1: by auto => /> /#.
 
-swap {1} 7 1.
-seq 7 1 : (#pre /\ 
+seq 3 1 : (#pre /\ 
            (forall k, 0<=k<32 => buf{1}.[k] = m{2}.[k]) /\
            (forall k, 0<=k<32 => kr{1}.[k] = _K{2}.[k]) /\
            (forall k, 0<=k<32 => kr{1}.[k+32] = r{2}.[k])).
 ecall {1} (sha3_512A_A64_ph buf{1}).
-wp; conseq (_: _ ==> 
-   (forall k, 0<=k<32 => buf{1}.[k] = m{2}.[k]) /\
-   (forall k, 32<=k<64 => buf{1}.[k] = mem.[_skp + 2336 + k - 32]) /\
-   (forall k, 0<=k<32 => buf{1}.[k] = aux{1}.[k])).
-+ auto => /> &1 &2; rewrite /load_array32 !tP => ?????????buf bvl bvh ; split.
++ auto => /> &1 &2; rewrite !tP => buf bvl bvh ; do split.
+  +  move => k kbl kbh; rewrite initiE 1:/# /= ifF 1:/# initiE 1:/# /#. 
   + move => k kbl kbh; rewrite initiE 1:/# /= kbh /= /G_mhpk; congr; congr;congr.
-    rewrite tP => i ib; rewrite initiE //= /#.
-    by rewrite tP => i ib; rewrite !initiE  /#. 
+    + rewrite tP => i ib; rewrite initiE 1:/# /= initiE  1:/# /= ifF 1: /# initiE /#.
+    rewrite tP => i ib; rewrite initiE 1:/# /= initiE  1:/# /= ifT 1: /# initiE 1:/# /= initiE 1:/# /=.
+    rewrite /get8 initiE 1:/# /= initiE 1:/# /= /get64 /(\bits8) wordP => *.
+    rewrite initiE 1:/# /= /init8 /get64_direct /pack8_t initiE 1:/# /= initiE 1:/# /= initiE 1:/# /= initiE 1:/# /= /#.
   + move => k kbl kbh; rewrite initiE 1:/# /= ifF 1:/# /= /G_mhpk; congr; congr;congr.
-    rewrite tP => i ib; rewrite initiE //= /#.
-    by rewrite tP => i ib; rewrite !initiE  /#. 
-while {1} (0<=i{1}<=4 /\ inc{1} = 4  /\ to_uint hp{1} = _skp + 2336 /\ Glob.mem{1} = mem /\
-             valid_ptr _skp (384*3 + 384*3 + 32 + 32 + 32+ 32) /\
-             (forall (k : int), 32 <= k && k < 32 + 8*i{1} => buf{1}.[k] = mem.[_skp + 2336 + k - 32]) /\
-             forall (k : int), 0 <= k && k < 32 => buf{1}.[k] = aux{1}.[k]) (4 - i{1}); last first. 
-  + auto => /> &1 &2; rewrite /valid_ptr => ???????? /=.
-    have -> /= : cph{2} = (cph{2}.`1,cph{2}.`2) by smt().
-    rewrite /load_array960 /load_array128 !tP => [#] cph1v cph2v.
-    do split.
-    + by rewrite /(`|>>`) /(`<<`) /= to_uintD_small of_uintK /= /#. 
-    + by smt().
-    + by move => k kbl kbh; rewrite initiE /= /#.
-    by smt().
-  move => *; auto => /> &hr ????????; do split; 1..2,5: by smt().
-  + move => k kbl kbh; rewrite initiE //= 1:/#.
-    rewrite /storeW64 /loadW64 /stores  /=. 
-    rewrite WArray64.WArray64.get8_set64_directE 1..2:/#.
-    case (32 + 8 * i{hr} <= k && k < 32 + 8 * i{hr} + 8).
-    + by move => *; rewrite pack8bE 1:/# initiE /= 1:/# to_uintD_small /= of_uintK /= modz_small /#. 
-    by move => *; rewrite /WArray64.WArray64.get8 WArray64.WArray64.initiE /= /#.  
-  move => k kbl kbh; rewrite initiE /= 1:/# WArray64.WArray64.get8_set64_directE 1..2:/#. 
-  case (32 + 8 * i{hr} <= k && k < 32 + 8 * i{hr} + 8).
-  + by move => *; rewrite pack8bE 1:/# initiE /= 1:/# to_uintD_small /= of_uintK /= modz_small /#. 
-  by move => *; rewrite /WArray64.WArray64.get8 WArray64.WArray64.initiE /= /#.  
-  
-swap {2} 1 1.  
-seq 4 1 : (#pre /\ to_uint s_skp{1} = _skp /\ 
-           ctpc{1} = Array1088.init (fun i => if i < 960 then c{2}.`1.[i] else c{2}.`2.[i-960])).
-+ wp;call (mlkem_correct_enc_1_avx2 mem (_skp + 1152)).
+    + rewrite tP => i ib; rewrite initiE 1:/# /= initiE  1:/# /= ifF 1: /# initiE /#.
+    rewrite tP => i ib; rewrite initiE 1:/# /= initiE  1:/# /= ifT 1: /# initiE 1:/# /= initiE 1:/# /=.
+    rewrite /get8 initiE 1:/# /= initiE 1:/# /= /get64 /(\bits8) wordP => *.
+    rewrite initiE 1:/# /= /init8 /get64_direct /pack8_t initiE 1:/# /= initiE 1:/# /= initiE 1:/# /= initiE 1:/# /= /#.
 
-  auto => /> &1 &2 ???????; rewrite /load_array1152 /load_array32 /load_array960 !tP => ?????; do split; 1..2: by smt().
-  + by move => i ib; rewrite initiE /= /#.
-  + by rewrite /(`|>>`) /(`<<`) /= to_uintD_small of_uintK /= /#. 
-  + by move => i ib; rewrite initiE /= /#.
-  move => /= ? ? bufv ? krv rl rr H. 
-  rewrite (_: rr = (rr.`1,rr.`2)) 1:/# /= in H.
-  rewrite tP => i ib.
-  rewrite !initiE //=. by  smt(Array128.initiE Array960.initiE).
+swap {2} 1 1.
 
-sp 3 0; seq 1 0 : (#pre /\ 
+seq 1 1 : (#pre /\ 
+           ctc{1} = Array1568.init (fun i => if i < 1408 then c{2}.`1.[i] else c{2}.`2.[i-1408])).
+print mlkem_correct_enc_1_avx2.
++ wp;ecall (mlkem_correct_enc_1_avx2 (Array1568.init (fun (i : int) => sk{1}.[4 * 384 + i]))).
+
+  auto => /> &1 &2; rewrite !tP => ??????; do split.
+  + by move => i ib; rewrite initiE /= /#.
+  + by move => i ib; rewrite initiE /= /#.
+  + move => i ib; rewrite initiE /= 1:/# initiE /= 1:/#;smt(Array1536.initiE).
+  + move => i ib; rewrite initiE /= 1:/# initiE /= 1:/#;smt(Array32.initiE).
+  move => /= ?  bufv ? krv rl [rr1 rr2] /=;rewrite !tP => H. 
+  by move => *;rewrite !initiE 1:/# /=; by  smt(Array160.initiE Array1408.initiE).
+
+seq 1 0 : (#pre /\ 
                   (c{2}  = cph{2} => cnd{1} = W64.of_int 0) /\
                   (c{2}  <> cph{2} => cnd{1} = W64.of_int 1)).
-+  conseq (_: _ ==> (c{2}  = cph{2} => cnd{1} = W64.of_int 0) /\
-                  (c{2}  <> cph{2} => cnd{1} = W64.of_int 1)); 1: smt(). 
-   ecall {1} (verify_correct mem _ctp ctpc{1}).
-   auto => /> &1 &2; rewrite /load_array960 /load_array128 !tP.
-   move  => ????????cphv????rst Heq Hdiff.
+   ecall {1} (verify_correct ct{1} ctc{1}). 
+   auto => /> &1 &2; rewrite !tP.
+   move  => ??cphv???rst Heq Hdiff. 
    rewrite (_: cph{2} = (cph{2}.`1, cph{2}.`2)) /= in cphv; 1: by smt().
    move : cphv;rewrite !tP ; move => [cphv1 cphv2].
    split.
    + move => ceq; rewrite (Heq _); last by done.
      move => i0 ib; rewrite !initiE //=. 
-     case (i0 < 960).
+     case (i0 < 1408).
      + by move => ibb; rewrite ceq cphv1 1: /# initiE /= /#.
      by move => ibb; rewrite ceq cphv2 1: /# initiE /= /#. 
-   move => neq;rewrite Hdiff. 
-   have : exists i0, 0<= i0 < 1088 /\ 
-     (Array1088.init (fun (i1 : int) => loadW8 mem (to_uint s_ctp{1} + i1))).[i0] <>
-     (Array1088.init (fun (i1 : int) => if i1 < 960 then c{2}.`1.[i1] else c{2}.`2.[i1 - 960])).[i0]; last by smt().
+   move => neq;rewrite Hdiff.
+   have : exists i0, 0<= i0 < 1568 /\ 
+     ct{1}.[i0] <>
+     (Array1568.init (fun (i1 : int) => if i1 < 1408 then c{2}.`1.[i1] else c{2}.`2.[i1 - 1408])).[i0]; last by smt().
    case (c{2}.`1 <> cph{2}.`1).
    + move => neq1. rewrite tP in neq1.   
-     have [k kb] : exists k, 0<=k<960 /\ c{2}.`1.[k] <> cph{2}.`1.[k] by smt().
+     have [k kb] : exists k, 0<=k<1408 /\ c{2}.`1.[k] <> cph{2}.`1.[k] by smt().
      exists k; split; 1: by smt().
-     rewrite !initiE /= 1,2:/#. 
+     rewrite initiE /= 1:/#. 
      move : (cphv1 k _); 1: smt().
      by rewrite initiE /= /#.
    + move => eq1. 
      have neq2 : c{2}.`2 <> cph{2}.`2 by move : neq eq1; smt().
      rewrite tP in neq2.   
-     have [k kb] : exists k, 0<=k<128 /\ c{2}.`2.[k] <> cph{2}.`2.[k] by smt().
-     exists (k + 960); split; 1: by smt().
-     rewrite !initiE /= 1,2:/#. 
+     have [k kb] : exists k, 0<=k<160 /\ c{2}.`2.[k] <> cph{2}.`2.[k] by smt().
+     exists (k + 1408); split; 1: by smt().
+     rewrite initiE /= 1:/#. 
      move : (cphv2 k _); 1: smt().
      by rewrite initiE /= /#.
   done.
 
 
-ecall {1} (cmov_correct (to_uint shkp{1}) (Array32.init (fun (i_0 : int) => kr{1}.[0 + i_0])) cnd{1} Glob.mem{1}).
+ecall {1} (cmov_correct shk{1} (Array32.init (fun (i : int) => kr{1}.[0 + i])) cnd{1}).
+wp;ecall{1} (shake256_A32_A1600_ph zp_ct{1}).
 
-wp;ecall{1} (shake256_M32__M32_M1088_ph  Glob.mem{1} (to_uint shkp{1}) (to_uint zp{1}) (to_uint ctp{1})).
-
-+ auto => /> &1 &2 ???????; rewrite /load_array1152 /load_array32 !tP => ?cphv????ceq cdif.
-do split;1,2:
-  by rewrite /(`|>>`) /(`<<`) /= to_uintD_small of_uintK /= /#. 
-move => ??????mm0 tt0 hashv;do split.
-+ move => badc mm back c0 c1;split.
-  + by move : back tt0 => /#.
-  + have -> : (init (fun (i0 : int) => mm.[to_uint shkp{1} + i0]))%Array32 =
-              (init (fun (i0 : int) => mm0.[to_uint shkp{1} + i0]))%Array32.
-    move : (c1 (cdif badc)).
++ auto => /> &1 &2; rewrite  !tP =>??.
+  have ->/= : (cph{2} = (cph{2}.`1,cph{2}.`2)) by smt(). 
+  move =>[#]; rewrite !tP => cphv1 cphv2 ???ceq cdif.
+do split. 
++ move => badc back c0 c1.
+  +  move : (c1 (cdif badc)).
     rewrite !tP => H k kb.
-    by rewrite (H k kb) !initiE 1,2:/# /= /loadW8 /loads.
-  rewrite hashv /J;congr.
-  + rewrite tP => k kb; rewrite !initiE 1,2:/# /=.
-    by rewrite /(`|>>`) /(`<<`) /= to_uintD_small of_uintK /= /#. 
-  rewrite (_: cph{2} = (cph{2}.`1, cph{2}.`2)) 1: /# /=.
-  rewrite (_: cph{2} = (cph{2}.`1, cph{2}.`2)) 1: /# /= in cphv.
-  by move : cphv => [-> ->]; rewrite /load_array960 /load_array128 /#.
+    rewrite (H k kb) !initiE 1,2:/# /=.
+    rewrite /J; congr; congr;congr;congr.
+    + congr;rewrite tP => kk kkb; rewrite !initiE 1..3:/# /= ifF 1:/# initiE 1:/# /=kkb /= initiE 1:/#.
+      rewrite /get8 initiE 1:/# /= initiE 1:/# /= /get64 /(\bits8) wordP => *.
+    rewrite initiE 1:/# /= /init8 /get64_direct /pack8_t initiE 1:/# /= initiE 1:/# /= initiE 1:/# /= initiE 1:/# /= /#.
+    + congr;rewrite tP => kk kkb; rewrite !initiE 1:/# /= initiE 1:/# /= ifT 1:/# /= initiE 1:/# /=.
+      rewrite /get8 initiE 1:/# /= initiE 1:/# /= /get64 /(\bits8) wordP => *.
+    rewrite initiE 1:/# /= /init8 /get64_direct /pack8_t initiE 1:/# /= initiE 1:/# /= initiE 1:/# /=.
+    smt(Array1408.initiE Array160.initiE).
 
-move => goodc mm back c0 c1;split.
-  + by move : back tt0 => /#.
+  rewrite tP => kk kkb; rewrite !initiE 1:/# /= initiE 1:/# /= ifT 1:/# /= initiE 1:/# /=.
+      rewrite /get8 initiE 1:/# /= initiE 1:/# /= /get64 /(\bits8) wordP => *.
+    rewrite initiE 1:/# /= /init8 /get64_direct /pack8_t initiE 1:/# /= initiE 1:/# /= initiE 1:/# /=.
+    smt(Array1408.initiE Array160.initiE).
+
+move => goodc  back c0 c1.
   + move : (c0 (ceq goodc)).
     rewrite !tP => H k kb.
     by rewrite (H k kb) initiE /#.
